src/Within.v
@@ -1,0 +1,114 @@
+Require Import
+  Here.Nomega
+  Here.Heap
+  Here.HeapADT
+  Here.FMapExt
+  Here.Relations
+  Here.MemoryBlockC
+  Coq.FSets.FMapFacts
+  Coq.Structures.DecidableTypeEx.
+
+Module Within (Mem : Memory) (M : WSfun N_as_DT).
+
+Module Import O := MemoryBlockC Mem M.
+Import A.
+Import A.H.
+
+Module X := FMapExt N_as_DT M.
+Include X.
+
+Definition within_allocated_mem (n : N) :=
+  fun (addr : M.key) (blk : MemoryBlockC) => addr + memCSize blk <=? n.
+
+Program Instance within_allocated_mem_Proper :
+  Proper (eq ==> eq ==> eq ==> eq) within_allocated_mem.
+Obligation 1. relational; subst; reflexivity. Qed.
+
+Lemma within_allocated_mem_add : forall n x k e,
+  within_allocated_mem n k e = true
+    -> 0 < x
+    -> within_allocated_mem (n + x) k e = true.
+Proof.
+  unfold within_allocated_mem; intros.
+  undecide.
+  apply Nle_add_plus; trivial.
+Qed.
+
+Lemma within_allocated_mem_at_end : forall n x d,
+   within_allocated_mem (n + x) n {| memCSize := x; memCData := d |} = true.
+Proof.
+  unfold within_allocated_mem; simpl; intros.
+  apply N.leb_refl.
+Qed.
+
+Corollary Proper_within : forall pos,
+   Proper (eq ==> eq ==> eq)
+          (fun b e => Decidable_witness (P:=within b (memCSize e) pos)).
+Proof. intros; relational; subst; reflexivity. Qed.
+
+Definition withinMemBlock (pos : N) (b : N) (e : MemoryBlock) : Prop :=
+  within b (memSize e) pos.
+
+Definition withinMemBlockC (pos : N) (b : N) (e : MemoryBlockC) : bool :=
+  Decidable_witness (P:=within b (memCSize e) pos).
+
+Global Program Instance withinMemBlock_Proper :
+  Proper (N.eq ==> eq ==> eq ==> eq) withinMemBlock.
+Obligation 1.
+  relational.
+  subst.
+  rewrite H.
+  reflexivity.
+Qed.
+
+Global Program Instance withinMemBlockC_Proper :
+  Proper (N.eq ==> eq ==> eq ==> eq) withinMemBlockC.
+Obligation 1.
+  relational.
+  subst.
+  rewrite H.
+  reflexivity.
+Qed.
+
+Open Scope lsignature_scope.
+
+Global Program Instance withinMemBlock_AbsR :
+  withinMemBlock [R eq ==> eq ==> MemoryBlock_AbsR ==> boolR]
+  withinMemBlockC.
+Obligation 1.
+  relational; subst;
+  unfold withinMemBlock, withinMemBlockC;
+  split; intros.
+    apply within_reflect in H.
+    rewrite <- (proj1 H1).
+    assumption.
+  simpl in H.
+  apply within_reflect.
+  rewrite (proj1 H1).
+  assumption.
+Qed.
+
+Global Program Instance withinMemBlock_AbsR_applied (pos : N) :
+  withinMemBlock pos [R eq ==> MemoryBlock_AbsR ==> boolR]
+  withinMemBlockC pos.
+Obligation 1. apply withinMemBlock_AbsR; reflexivity. Qed.
+
+Notation "f \oo g" := (fun x y => f (g x y)) (at level 90).
+
+Lemma withinMemAbsR : forall base blk cblk pos,
+  withinMemBlock pos base blk
+    -> MemoryBlock_AbsR blk cblk
+    -> withinMemBlockC pos base cblk = true.
+Proof.
+  intros.
+  unfold withinMemBlock, withinMemBlockC in *; simpl in *.
+  apply within_reflect in H.
+  destruct H0 as [H0 _]; rewrite <- H0.
+  assumption.
+Qed.
+
+Hint Resolve within_allocated_mem_Proper.
+Hint Resolve withinMemBlock_Proper.
+Hint Resolve withinMemBlockC_Proper.
+
+End Within.
